compiler/backend/closLangScript.sml
@@ -98,6 +98,8 @@ Datatype:
      | RefArray      (* makes an array by replicating a value *)
      | DerefByte     (* loads a byte from a byte array *)
      | UpdateByte    (* updates a byte array *)
+     | DerefBit      (* read a bit from a byte array *)
+     | SetBit bool   (* set a bit of a byte array *)
      | ConcatByteVec (* concatenate list of byte vectors *)
      | CopyByte bool (* copy a slice of a byte array, T means target should be allocated *)
      | FromListByte  (* convert list of chars to ByteVector *)
@@ -183,6 +185,7 @@ Definition pure_op_def:
     | MemOp (RefByte _) => F
     | MemOp RefArray => F
     | MemOp UpdateByte => F
+    | MemOp (SetBit _) => F
     | MemOp (CopyByte F) => F
     | MemOp XorByte => F
     | MemOp Ref => F
